spec serialize_cbor_map

src/cbor/spec/raw/CBOR.Spec.API.Format.fst
@@ -92,3 +92,174 @@ let cbor_det_serialize_array_length_gt_list l =
   R.mk_cbor_eq x;
   R.mk_det_raw_cbor_mk_cbor x;
   assert (R.mk_det_raw_cbor (pack (CArray l)) == x)
+
+let cbor_det_serialize_map m =
+  R.serialize_cbor_map (R.mk_det_raw_cbor_map_raw m)
+
+let cbor_det_serialize_map_empty () =
+  R.serialize_cbor_map_nil ()
+
+let cbor_det_serialize_map_singleton key value =
+  R.mk_det_raw_cbor_map_raw_singleton key value;
+  R.serialize_cbor_map_singleton (R.mk_det_raw_cbor key) (R.mk_det_raw_cbor value)
+
+#push-options "--z3rlimit 32"
+
+#restart-solver
+
+let rec cbor_det_serialize_map_length_union_disjoint_eq
+  (m1: cbor_map)
+  (l2: list (cbor & cbor))
+  (m2: cbor_map)
+: Lemma
+  (requires (
+    List.Tot.length l2 == cbor_map_length m2 /\
+    List.Tot.no_repeats_p (List.Tot.map fst l2) /\
+    (forall x . List.Tot.assoc x l2 == cbor_map_get m2 x) /\
+    cbor_map_disjoint m1 m2
+  ))
+  (ensures (
+    Seq.length (cbor_det_serialize_map (cbor_map_union m1 m2)) == Seq.length (cbor_det_serialize_map m1) + Seq.length (R.serialize_cbor_map (List.Tot.map R.mk_det_raw_cbor_map_entry l2))
+  ))
+  (decreases l2)
+= match l2 with
+  | [] ->
+    R.serialize_cbor_map_nil ();
+    assert (cbor_map_equal m2 cbor_map_empty)
+  | (k, v) :: q ->
+    let ms = cbor_map_singleton k v in
+    let m1' = cbor_map_union m1 ms in
+    let m2' = cbor_map_sub m2 ms in
+    assert (cbor_map_equal (cbor_map_union m1 m2) (cbor_map_union m1' m2'));
+    R.serialize_cbor_map_cons (R.mk_det_raw_cbor k) (R.mk_det_raw_cbor v) (List.Tot.map R.mk_det_raw_cbor_map_entry q);
+    List.Tot.assoc_mem k q;
+    assert (cbor_map_equal m2 (cbor_map_union m2' ms));
+    cbor_map_length_disjoint_union m2' ms;
+    cbor_map_length_singleton k v;
+    let kr = R.mk_det_raw_cbor k in
+    let vr = R.mk_det_raw_cbor v in
+    assert (R.serialize_cbor_map (List.Tot.map R.mk_det_raw_cbor_map_entry l2) == (R.serialize_cbor kr `Seq.append` R.serialize_cbor vr) `Seq.append` R.serialize_cbor_map (List.Tot.map R.mk_det_raw_cbor_map_entry q)
+    );
+    assert (Seq.length (R.serialize_cbor_map (List.Tot.map R.mk_det_raw_cbor_map_entry l2)) == Seq.length (R.serialize_cbor kr) + Seq.length (R.serialize_cbor vr) + Seq.length (R.serialize_cbor_map (List.Tot.map R.mk_det_raw_cbor_map_entry q))
+    );
+    cbor_det_serialize_map_length_union_disjoint_eq m1' q m2';
+    R.mk_det_raw_cbor_map_raw_snoc m1 k v;
+    let l1 = R.mk_det_raw_cbor_map_raw m1 in
+    let kv = (R.mk_det_raw_cbor k, R.mk_det_raw_cbor v) in
+    R.mk_det_raw_cbor_map_raw_assoc m1 k;
+    R.list_setoid_assoc_sorted_optimal R.deterministically_encoded_cbor_map_key_order (R.mk_det_raw_cbor k) l1;
+    List.Tot.assoc_mem (R.mk_det_raw_cbor k) l1;
+    RF.cbor_map_insert_sorted l1 kv;
+    RF.serialize_cbor_map_insert_length l1 kv;
+    assert (Some? (RF.cbor_map_insert l1 kv));
+    let Some l1' = RF.cbor_map_insert l1 kv in
+    assert (cbor_det_serialize_map m1' == R.serialize_cbor_map l1');
+    ()
+
+#pop-options
+
+let cbor_det_serialize_map_length_eq
+  (l2: list (cbor & cbor))
+  (m2: cbor_map)
+: Lemma
+  (requires (
+    List.Tot.length l2 == cbor_map_length m2 /\
+    List.Tot.no_repeats_p (List.Tot.map fst l2) /\
+    (forall x . List.Tot.assoc x l2 == cbor_map_get m2 x)
+  ))
+  (ensures (
+    Seq.length (cbor_det_serialize_map (m2)) == Seq.length (R.serialize_cbor_map (List.Tot.map R.mk_det_raw_cbor_map_entry l2))
+  ))
+= cbor_det_serialize_map_length_union_disjoint_eq cbor_map_empty l2 m2;
+  cbor_det_serialize_map_empty ()
+
+let rec cbor_map_to_list
+  (m: cbor_map)
+  (l: list cbor)
+: Tot (list (cbor & cbor))
+= match l with
+  | [] -> []
+  | k :: q ->
+    begin match cbor_map_get m k with
+    | None -> cbor_map_to_list m q
+    | Some v -> (k, v) :: cbor_map_to_list m q
+    end
+
+let rec cbor_map_to_list_map_fst
+  (m: cbor_map)
+  (l: list cbor)
+: Lemma
+  (requires (
+    forall x . List.Tot.memP x l ==> cbor_map_defined x m
+  ))
+  (ensures (
+    let l' = cbor_map_to_list m l in
+    List.Tot.map fst l' == l
+  ))
+= match l with
+  | [] -> ()
+  | _ :: q -> cbor_map_to_list_map_fst m q
+
+let rec cbor_map_to_list_assoc
+  (m: cbor_map)
+  (l: list cbor)
+  (k: cbor)
+: Lemma
+  (requires (
+    List.Tot.memP k l /\
+    cbor_map_defined k m
+  ))
+  (ensures (
+    let l' = cbor_map_to_list m l in
+    List.Tot.assoc k l' == cbor_map_get m k
+  ))
+= match l with
+  | [] -> ()
+  | k' :: q ->
+    if k = k'
+    then ()
+    else cbor_map_to_list_assoc m q k
+
+let cbor_map_to_list_assoc'
+  (m: cbor_map)
+  (l: list cbor)
+  (k: cbor)
+: Lemma
+  (ensures (
+    List.Tot.memP k l /\
+    cbor_map_defined k m
+  ) ==> (
+    let l' = cbor_map_to_list m l in
+    List.Tot.assoc k l' == cbor_map_get m k
+  ))
+= Classical.move_requires (cbor_map_to_list_assoc m l) k
+
+let cbor_map_to_list_correct
+  (m: cbor_map)
+  (l: list cbor)
+: Lemma
+  (requires (
+    (forall x . List.Tot.memP x l <==> cbor_map_defined x m) /\
+    List.Tot.no_repeats_p l
+  ))
+  (ensures (
+    let l' = cbor_map_to_list m l in
+    (forall x . List.Tot.assoc x l' == cbor_map_get m x)
+  ))
+= let l' = cbor_map_to_list m l in
+  Classical.forall_intro (cbor_map_to_list_assoc' m l);
+  cbor_map_to_list_map_fst m l;
+  Classical.forall_intro (fun x -> List.Tot.assoc_mem x l')
+
+let cbor_det_serialize_map_append_length m1 m2 =
+  let l = cbor_map_key_list m2 in
+  let l' = cbor_map_to_list m2 l in
+  cbor_map_to_list_map_fst m2 l;
+  cbor_map_to_list_correct m2 l;
+  cbor_det_serialize_map_length_union_disjoint_eq m1 l' m2;
+  cbor_det_serialize_map_length_eq l' m2
+
+let cbor_det_serialize_map_length_gt_list l =
+  R.mk_cbor_eq_map (pack (CMap l));
+  R.cbor_serialize_map_length_gt_list (R.mk_raw_uint64 (U64.uint_to_t (cbor_map_length l))) (R.mk_det_raw_cbor_map_raw l);
+  ()
